wip: saving current state

fairness/model_plug.v
@@ -3,36 +3,75 @@ From iris.base_logic.lib Require Import invariants.
 From iris.proofmode Require Import tactics.
 
 Section ModelPlug.
-  (* Context `{Countable G}.  *)
-  (* Context `{iLM: LiveModel G iM LSI}. *)
   Context `{EM: ExecutionModel Λ M__glob}.
   Context `{eGS: em_GS Σ}. 
-  Context `{invGS_gen HasNoLc Σ}.
 
   Context {M: FairModel}.
-  Context {msi: fmstate M -> iProp Σ}. 
-  (* Context `{Countable (locale Λ)}.  *)
-  (* Context {PMPP: @PartialModelPredicatesPre G _ _ Σ iM}. *)
+  Context {msi: fmstate M -> iProp Σ}.
 
-  Context (relies_on: locale Λ -> fmrole M -> iProp Σ).
-  Context (ε: coPset).
+  Definition local_rule (P Q: iProp Σ) (ρ: fmrole M): iProp Σ :=
+    □ (∀ (δ: fmstate M), P ∗ msi δ ==∗ ∃ δ', Q ∗ msi δ' ∗ ⌜ fmtrans M δ (Some ρ) δ' ⌝). 
 
-  (* Definition model_lifted_step (P Q: iProp Σ) *)
-  (*   (τ: locale Λ) (extr: execution_trace Λ) (auxtr: auxiliary_trace M__glob) c2 *)
+  Section MP.
+    Context `{invGS_gen HasNoLc Σ}.
+    (* Context (lift_ctx: iProp Σ). *)
+    Context (ε: coPset).
 
-  Definition model_plugged: iProp Σ :=
-    ∀ P Q (gl: fmrole M),
-       □ ((∀ (δ: fmstate M), P ∗ msi δ ==∗ ∃ δ', Q ∗ msi δ' ∗ ⌜ fmtrans M δ (Some gl) δ' ⌝) →
-      (∀ (τ: locale Λ) (extr: execution_trace Λ) (auxtr: auxiliary_trace M__glob) c2,
-        relies_on τ gl ∗
-        P ∗ 
-        em_msi (trace_last extr) (trace_last auxtr) (em_GS0 := eGS) ∗
-        ⌜ locale_step (trace_last extr) (Some τ) c2 ⌝ 
-        ={ ε }=∗
-         ∃ (δ2 : M__glob) (ℓ : mlabel M__glob),
-         relies_on τ gl ∗
-         Q ∗
-         em_msi c2 δ2 (em_GS0 := eGS) ∗
-         ⌜em_valid_state_evolution_fairness (extr :tr[ Some τ ]: c2) (auxtr :tr[ ℓ ]: δ2)⌝)).
+    Definition role_lift (τ: locale Λ) (gl: fmrole M) (lift_ctx: iProp Σ): iProp Σ :=
+      ∀ P Q, 
+        □ (local_rule P Q gl -∗
+           ∀ (extr: execution_trace Λ) (auxtr: auxiliary_trace M__glob) c2,
+             lift_ctx ∗
+             P ∗ 
+             em_msi (trace_last extr) (trace_last auxtr) (em_GS0 := eGS) ∗
+             ⌜ locale_step (trace_last extr) (Some τ) c2 ⌝ 
+             ={ ε }=∗
+             ∃ (δ2 : M__glob) (ℓ : mlabel M__glob),
+             lift_ctx ∗
+             Q ∗
+             em_msi c2 δ2 (em_GS0 := eGS) ∗
+             ⌜em_valid_state_evolution_fairness (extr :tr[ Some τ ]: c2) (auxtr :tr[ ℓ ]: δ2)⌝).
+
+    Global Instance RL_pers: forall τ ρ lc, Persistent (role_lift τ ρ lc).
+    Proof. apply _. Qed. 
+
+  End MP.
+
+  Section CWP.
+    Context `{!irisG Λ M__glob Σ}.
+        
+    Let RL := @role_lift iris_invGS. 
+                
+    Definition cwp (e: expr Λ) (Φ: val Λ -> iProp Σ) (s: stuckness) (ε__wp ε__lift: coPset) (τ: locale Λ) (ρ: fmrole M): iProp Σ :=
+      ∀ (lift_ctx: iProp Σ), lift_ctx -∗ RL ε__lift τ ρ lift_ctx  -∗ 
+                              WP e @ s ; τ ; ε__wp {{ v, Φ v ∗ lift_ctx }}. 
+
+  End CWP.
 
 End ModelPlug.
+
+
+Lemma cwp_convert
+  `{EM: ExecutionModel Λ M__glob}
+  `{!irisG Λ M__glob Σ}
+  `{eGS: em_GS Σ}
+   {M M': FairModel}
+   {msi: fmstate M -> iProp Σ} {msi': fmstate M' -> iProp Σ}
+   (CWP := @cwp _ _ EM _ eGS _ msi _)
+   (CWP' := @cwp _ _ EM _ eGS _ msi' _)
+   (RL := @role_lift _ _ EM Σ eGS _ msi iris_invGS)
+   (RL' := @role_lift _ _ EM Σ eGS _ msi' iris_invGS)
+   (e: expr Λ) τ (Φ Φ': val Λ -> iProp Σ) s ε__wp ε__lift ε__lift' ρ ρ':
+      ⊢ CWP' e Φ' s ε__wp ε__lift' τ ρ' -∗
+        (∀ LC, LC -∗ RL ε__lift τ ρ LC -∗ ∃ LC', LC' ∗ RL' ε__lift' τ ρ' LC' ∗ (∀ v,  Φ' v ∗ LC' -∗ Φ v ∗ LC)) -∗
+        CWP e Φ s ε__wp ε__lift τ ρ.
+Proof.
+  iIntros "CWP' CONV".
+  rewrite /CWP /cwp. iIntros (LC) "LC RL".
+  iSpecialize ("CONV" $! _ with "LC RL").
+  iDestruct "CONV" as (LC') "(LC' & RL' & CONV)".
+  iSpecialize ("CWP'" with "LC' RL'").
+  iApply (wp_strong_mono with "CWP'").
+  1, 2: reflexivity.
+  iIntros. iModIntro. by iApply "CONV".
+Qed. 
