fairness/heap_lang/model_logic.v
@@ -1,0 +1,112 @@
+From stdpp Require Import fin_maps.
+From iris.proofmode Require Import tactics.
+From iris.base_logic Require Export gen_heap.
+From trillium.fairness.heap_lang Require Import tactics notation sswp_logic.
+From trillium.fairness Require Import fairness resources fuel model_plug lm_fair.
+
+Section ModelLogic.
+
+  Context `{EM: ExecutionModel heap_lang M__glob}.   
+  Context `{hGS: @heapGS Σ _ EM}.
+  Let eGS := heap_fairnessGS.
+
+  Context {M: FairModel}.
+  Context {msi: fmstate M -> iProp Σ}. 
+
+  Let CWP := @cwp _ _ EM _ eGS _ msi _. 
+
+  Lemma cwp_model_sswp_step s tid ρ E ε__lift e Φ P Q:
+    TCEq (to_val e) None →
+    ε__lift ⊆ E ->
+    local_rule (msi := msi) P Q ρ -∗
+    ▷ P -∗
+    sswp s E e (λ e', Q -∗ CWP e' Φ s E ε__lift tid ρ) -∗
+    CWP e Φ s E ε__lift tid ρ.
+  Proof.
+    iIntros (Hval SUBM) "#RULE P SSWP". 
+    rewrite /CWP /cwp. iIntros (LC) "LC #LIFT".
+    
+    rewrite wp_unfold /wp_pre. rewrite /sswp. simpl. rewrite Hval.
+    iIntros (extr atr K tp1 tp2 σ1 Hvalid Hloc Hexend) "(% & Hsi & Hmi)".
+
+    iMod ("SSWP" with "Hsi") as (Hred) "Hwp". iIntros "!>".
+    iSplitR; [by rewrite Hexend in Hred|]. iIntros (????). rewrite Hexend.
+    iMod ("Hwp" with "[//]") as "Hwp". iIntros "!>!>". iMod "Hwp". iIntros "!>".
+    iApply step_fupdN_intro; [done|]. iIntros "!>".
+    iMod "Hwp" as "[Hσ [Hwp ->]]".
+    rewrite /trace_ends_in in Hexend. rewrite -Hexend.
+
+    iApply fupd_mask_mono; eauto.
+    rewrite /role_lift.
+    iMod ("LIFT" with "RULE [LC P Hmi]") as (δ2 ℓ) "(LC & Q & MSI & %EV)". 
+    { iFrame. iPureIntro.
+      rewrite -Hloc. eapply locale_step_atomic; eauto. by apply fill_step. }
+
+    iSpecialize ("Hwp" with "Q LC [$]"). 
+    iModIntro. do 2 iExists _. iFrame.
+    iSplit; done.
+  Qed.
+
+  Lemma cwp_value s E ε__lift Φ ζ ρ e v : IntoVal e v → Φ v ⊢ CWP e Φ s E ε__lift ζ ρ.
+  Proof.
+    rewrite /CWP /cwp. iIntros (?) "? % ??".
+    iApply wp_value. iFrame.
+  Qed.
+
+Section ModelLogic.
+  Set Default Proof Using "Type".
+
+  Context `{EM: ExecutionModel heap_lang M}.   
+  Context `{hGS: @heapGS Σ _ EM}.
+  Let eGS := heap_fairnessGS.
+
+  Context `{Countable G}.
+  Context `{iLM: LiveModel G iM LSI}.
+  Context {LFP: LMFairPre iLM}.
+  Let LF := LM_Fair (LF := LFP). 
+  Context {fGS: @fairnessGS _ _ _ _ _ iLM Σ}. 
+
+  Let CWP := @cwp _ _ EM _ eGS LF (model_state_interp (LM := iLM)) _. 
+  
+  Notation "tid ↦M R" := (partial_mapping_is {[ tid := R ]}) (at level 33).
+  Notation "tid ↦m ρ" := (partial_mapping_is {[ tid := {[ ρ ]} ]}) (at level 33).
+  Notation "ρ ↦F f" := (partial_fuel_is {[ ρ := f ]}) (at level 33).
+
+
+  
+
+Lemma wp_step_model s tid ρ (f1 : nat) fs fr s1 s2 E ε__lift e Φ (g: G):
+  TCEq (to_val e) None →
+  fmtrans iM s1 (Some ρ) s2 →
+  iM.(live_roles) s2 ⊆ iM.(live_roles) s1 →
+  ρ ∉ dom fs →
+  ▷ frag_model_is s1 -∗
+  ▷ has_fuels g ↦M ({[ρ:=f1]} ∪ fmap S fs) -∗
+  ▷ frag_free_roles_are fr -∗
+  sswp s E e (λ e', frag_model_is s2 -∗
+                    g ↦M ({[ρ:=(iLM.(lm_fl) s2)]} ∪ fs) -∗
+                    frag_free_roles_are fr -∗
+                    WP e' @ s; tid; E {{ Φ }} ) -∗
+  (* WP e @ s; tid; E {{ Φ }}. *)
+  CWP e Φ s E ε__lift tid g.
+Proof.
+  iIntros (Hval Htrans Hlive Hdom) ">Hst >Hfuel1 >Hfr Hwp".
+  rewrite wp_unfold /wp_pre.
+  rewrite /sswp. simpl. rewrite Hval.
+  iIntros (extr atr K tp1 tp2 σ1 Hvalid Hloc Hexend) "(% & Hsi & Hmi)".
+  iMod ("Hwp" with "Hsi") as (Hred) "Hwp". iIntros "!>".
+  iSplitR; [by rewrite Hexend in Hred|]. iIntros (????). rewrite Hexend.
+  iMod ("Hwp" with "[//]") as "Hwp". iIntros "!>!>". iMod "Hwp". iIntros "!>".
+  iApply step_fupdN_intro; [done|]. iIntros "!>".
+  iMod "Hwp" as "[Hσ [Hwp ->]]".
+  iDestruct (model_agree' with "Hmi Hst") as %Hmeq. iFrame.
+  rewrite /trace_ends_in in Hexend. rewrite -Hexend.
+  iMod (update_model_step with "Hfuel1 Hst Hmi") as
+    (δ2 Hvse) "(Hfuel & Hst & Hmod)"; eauto.
+  - rewrite -Hloc. eapply locale_step_atomic; eauto. by apply fill_step.
+  - iModIntro; iExists δ2, (Take_step ρ tid). rewrite big_sepL_nil. iFrame.
+    iSplit; [done|]. iDestruct ("Hwp" with "Hst Hfuel Hfr") as "Hwp". by iFrame.
+Qed.
+
+
+End ModelLogic.
