fairness/lm_rules/resources_updates.v
@@ -1,0 +1,344 @@
+From iris.algebra Require Import auth gmap gset excl.
+From iris.proofmode Require Import tactics.
+From trillium.fairness Require Import fuel resources.
+
+Section AuxDefs.
+  Context `{Countable G}. 
+  Context `{LM: LiveModel G M LSI}.
+
+  Definition valid_new_fuelmap (fs1 fs2: gmap (fmrole M) nat) (s1 s2: M) (ρ: fmrole M) :=
+    (ρ ∈ live_roles _ s2 -> oleq (fs2 !! ρ) (Some (LM.(lm_fl) s2))) ∧
+    (ρ ∉ live_roles _ s2 -> ρ ∈ dom fs1 ∩ dom fs2 -> oleq (fs2 !! ρ) (fs1 !! ρ)) ∧
+    ρ ∈ dom fs1 ∧
+    (forall ρ', ρ' ∈ dom fs2 ∖ dom fs1 -> oleq (fs2 !! ρ') (Some $ LM.(lm_fl) s2)) ∧
+    (forall ρ', ρ ≠ ρ' -> ρ' ∈ dom fs1 ∩ dom fs2 -> oless (fs2 !! ρ') (fs1 !! ρ')) ∧
+    (dom fs1 ∖ {[ ρ ]}) ∪ (live_roles _ s2 ∖ live_roles _ s1) ⊆ dom fs2 ∧
+    dom fs2 ⊆
+      (* new roles *) (live_roles _ s2 ∖ live_roles _ s1) ∪
+      (* surviving roles *) (live_roles _ s2 ∩ live_roles _ s1 ∩ dom fs1) ∪
+      (* already dead *) (dom fs1 ∖ live_roles _ s1) ∪
+      (* new deads *) ((live_roles _ s1 ∖ live_roles _ s2) ∩ dom fs1).
+
+  Definition fuel_apply (fs' F: gmap (fmrole M) nat) (LR: gset (fmrole M)):
+    gmap (fmrole M) nat :=
+    map_imap
+      (λ (ρ: fmrole M ) (fold : nat),
+       match decide (ρ ∈ dom fs') with
+       | left x => fs' !! ρ
+       | right _ => F !! ρ
+       end) (gset_to_gmap (0%nat) LR).
+
+  Definition update_fuel_resource 
+    (* (δ1: LiveState G M LSI) *) (F: gmap (fmrole M) nat)
+    (fs1 fs2: gmap (fmrole M) nat): gmap (fmrole M) nat :=
+    fuel_apply fs2 F ((dom F ∪ dom fs2) ∖ (dom fs1 ∖ dom fs2)).
+
+
+  (* (* TODO: refactor this? *) *)
+  Definition update_rmap (R: gmap (fmrole M) G) (ζ: G) (fs1 fs2: gmap (fmrole M) nat): gmap (fmrole M) G := 
+    map_imap (λ ρ' _, if decide (ρ' ∈ dom R) then R !! ρ' else Some ζ)
+      (gset_to_gmap 333 ((dom R ∪ dom fs2) ∖ (dom fs1 ∖ dom fs2))). 
+
+  Definition LSI_fuel_independent :=
+    forall S R F F',
+      LSI S R F -> LSI S R F'.
+
+  Definition fuel_reorder_preserves_LSI :=
+    forall S (R R': groups_map) F F',
+      dom F = dom F' ->
+      mapped_roles R = mapped_roles R' ->
+      dom F = mapped_roles R ->
+      LSI S R F -> LSI S R' F'. 
+
+  Definition fuel_drop_preserves_LSI S (rem: gset (fmrole M)) :=
+    forall (R: groups_map) F F',
+      (* let R' := filter (fun '(k, _) => k ∉ rem) R in *)
+      let R' := (fun rs => rs ∖ rem) <$> R in
+      LSI S R F -> LSI S R' F'. 
+
+  Definition model_step_preserves_LSI s1 ρ s2 fs1 fs2 :=
+    forall (R: groups_map) g F,
+      LSI s1 R F -> fmtrans M s1 (Some ρ) s2 ->
+      (* ls_mapping_impl R !! ρ = Some g -> *)
+      ρ ∈ default ∅ (R !! g) ->
+      LSI s2 (<[g:=dom fs2]> R) (update_fuel_resource F fs1 fs2). 
+
+End AuxDefs.
+
+
+Section Updates.
+  Context `{Countable G}. 
+  Context `{LM: LiveModel G M LSI}.
+  Context {Σ: gFunctors}. 
+  Context {fGS: @fairnessGS _ _ _ _ _ LM Σ}. 
+
+  Lemma update_model δ δ1 δ2:
+    auth_model_is δ1 -∗ frag_model_is δ2 ==∗ auth_model_is δ ∗ frag_model_is δ.
+  Proof.
+    iIntros "H1 H2". iCombine "H1 H2" as "H".
+    iMod (own_update with "H") as "[??]" ; eauto.
+    - by apply auth_update, option_local_update, (exclusive_local_update _ (Excl δ)).
+    - iModIntro. iFrame.
+  Qed.
+
+  Lemma update_free_roles rem FR fr1:
+    rem ⊆ fr1 ->
+    auth_free_roles_are FR -∗
+    frag_free_roles_are fr1 ==∗
+    auth_free_roles_are (FR ∖ rem) ∗
+    frag_free_roles_are (fr1 ∖ rem).
+  Proof.
+    iIntros (?) "HFR Hfr1".
+
+    iDestruct (free_roles_inclusion with "HFR Hfr1") as %Hincl.
+
+    replace FR with ((FR ∖ rem) ∪ rem); last first.
+    { rewrite difference_union_L. set_solver. }
+    replace fr1 with ((fr1 ∖ rem) ∪ rem); last first.
+    { rewrite difference_union_L. set_solver. }
+
+    iAssert (frag_free_roles_are (fr1 ∖ rem) ∗ frag_free_roles_are rem)%I with "[Hfr1]" as "[Hfr2 Hrem]".
+    { rewrite /frag_free_roles_are -own_op -auth_frag_op gset_disj_union //. set_solver. }
+
+    iCombine "HFR Hrem" as "H".
+    iMod (own_update with "H") as "[??]" ; eauto.
+    - apply auth_update, gset_disj_dealloc_local_update.
+    - iModIntro. iFrame. iApply (own_proper with "Hfr2").
+      do 2 f_equiv. set_solver.
+  Qed.
+
+  Lemma update_free_roles_strong fr1 fr2 FR'
+    (DISJ1: fr1 ## FR') (DISJ2: fr2 ## FR'):
+    auth_free_roles_are (fr1 ∪ FR') -∗
+    frag_free_roles_are fr1 ==∗
+    auth_free_roles_are (fr2 ∪ FR') ∗
+    frag_free_roles_are fr2.
+  Proof.
+    iIntros "HFR Hfr1".
+    iApply own_op. 
+    iMod (own_update with "[Hfr1 HFR]") as "?".
+    3: { done. }
+    2: { iApply own_op. iFrame. }
+    apply auth_update.
+    etrans.
+    { apply gset_disj_dealloc_local_update. }
+    rewrite difference_union_distr_l_L difference_diag_L union_empty_l_L.
+    rewrite difference_disjoint_L; auto.
+    etrans. 
+    - by apply gset_disj_alloc_local_update with (Z := fr2).
+    - eapply local_update_proper.
+      1: rewrite union_empty_r_L.
+      all: reflexivity.
+  Qed. 
+
+  Notation "tid ↦M R" := (frag_mapping_is {[ tid := R ]}) (at level 33).
+  Notation "tid ↦m ρ" := (frag_mapping_is {[ tid := {[ ρ ]} ]}) (at level 33).
+  Notation "ρ ↦F f" := (frag_fuel_is {[ ρ := f ]}) (at level 33).
+
+  Lemma update_fuel_delete ρ f F:
+    auth_fuel_is F -∗ ρ ↦F f ==∗ auth_fuel_is (delete ρ F).
+  Proof.
+    iIntros "Hafuel Hfuel".
+    iCombine "Hafuel Hfuel" as "H".
+    iMod (own_update with "H") as "H"; last first.
+    { iModIntro. iFrame. }
+    rewrite map_fmap_singleton fmap_delete.
+    eapply auth_update_dealloc.
+    apply delete_singleton_local_update.
+    typeclasses eauto.
+  Qed.
+
+  Lemma update_fuel fs fs' F:
+    let LR := (dom F ∪ dom fs') ∖ (dom fs ∖ dom fs') in
+    (fs ≠ ∅) ->
+    (dom fs' ∖ dom fs ∩ dom F = ∅) ->
+    auth_fuel_is F -∗
+    ([∗ map] ρ ↦ f ∈ fs, ρ ↦F f) ==∗
+      auth_fuel_is (fuel_apply fs' F LR) ∗
+      ([∗ map] ρ ↦ f ∈ fs', ρ ↦F f).
+  Proof.
+    iIntros (? Hnotemp Hdisj) "Hafuel Hfuel".
+    rewrite {1}/frag_fuel_is -big_opM_own //.
+    setoid_rewrite map_fmap_singleton.
+    rewrite -big_opM_auth_frag.
+    iCombine "Hafuel Hfuel" as "H".
+    iMod (own_update with "H") as "[A B]"; last first.
+    { iModIntro.
+      destruct (decide (fs' = ∅)) as [Heq|]; last first.
+      -  rewrite {1}/frag_fuel_is -big_opM_own //.
+         iSplitL "A"; done.
+      - rewrite Heq. iSplitL "A"; first done. done. }
+
+    simpl.
+    setoid_rewrite map_fmap_singleton.
+    rewrite -big_opM_auth_frag.
+
+    simpl.
+    apply auth_update.
+
+    apply local_update_discrete.
+
+    intros mf Hval Heq.
+    split.
+    { intros ρ. rewrite /fuel_apply lookup_fmap map_lookup_imap.
+      rewrite lookup_gset_to_gmap.
+      destruct (decide (ρ ∈ LR)).
+      - rewrite option_guard_True //=.
+        destruct (decide (ρ ∈ dom fs')) as [Hd|Hd].
+        + rewrite decide_True //=. apply elem_of_dom in Hd as [? Hsome].
+          rewrite Hsome //.
+        + rewrite decide_False //= -lookup_fmap. apply (Hval ρ).
+      - rewrite option_guard_False //=. }
+
+    intros ρ. rewrite /fuel_apply lookup_fmap map_lookup_imap.
+    rewrite lookup_gset_to_gmap.
+    rewrite -big_opM_fmap big_opM_singletons.
+    rewrite <-big_opM_fmap in Heq. setoid_rewrite big_opM_singletons in Heq.
+    destruct (decide (ρ ∈ LR)).
+    - rewrite option_guard_True //=.
+      destruct (decide (ρ ∈ dom fs')) as [Hd'|Hd'].
+      + rewrite decide_True //=. apply elem_of_dom in Hd' as [? Hsome].
+        rewrite Hsome //= lookup_opM.
+        rewrite lookup_fmap Hsome.
+        destruct mf as [mf|]; simpl; last done.
+        destruct (mf !! ρ) as [f|] eqn:Hlk; rewrite Hlk //.
+
+        assert (ρ ∈ dom F ∖ dom fs).
+        { eauto using elem_of_frame_excl_map. }
+        assert (ρ ∈ dom fs').
+        { apply elem_of_dom. eauto. }
+        set_solver.
+      + rewrite decide_False //= -lookup_fmap.
+        rewrite Heq.
+        destruct (decide (ρ ∈ dom fs)) as [Hd|Hd];
+          first set_solver.
+        pose proof Hd as Hd2. pose proof Hd' as Hd'2.
+        apply not_elem_of_dom in Hd2, Hd'2. rewrite !lookup_opM !lookup_fmap Hd2 Hd'2 //.
+    - rewrite option_guard_False //=.
+      rewrite lookup_opM lookup_fmap.
+      destruct mf as [mf|]; simpl.
+      + destruct (mf !! ρ) as [f|] eqn:Hlk; rewrite Hlk //.
+        * assert (ρ ∈ dom F ∖ dom fs).
+          { eauto using elem_of_frame_excl_map. }
+          set_solver.
+        * assert (Hnotin: ρ ∉ dom fs') by set_solver.
+          apply not_elem_of_dom in Hnotin. rewrite Hnotin //.
+      + assert (Hnotin: ρ ∉ dom fs') by set_solver.
+        apply not_elem_of_dom in Hnotin. rewrite Hnotin //.
+  Qed.
+
+  Lemma update_mapping ζ (R' : gset $ fmrole M) (R: gset (fmrole M)) m :
+    auth_mapping_is m -∗ ζ ↦M R ==∗ auth_mapping_is (<[ ζ := R' ]> m) ∗ ζ ↦M R'.
+  Proof.
+    iIntros "Hamap Hmap".
+    iCombine "Hamap Hmap" as "H".
+    iMod (own_update with "H") as "[A B]"; last first.
+    { iModIntro. iSplitL "A"; iFrame. }
+    rewrite !map_fmap_singleton fmap_insert.
+    eapply auth_update, singleton_local_update_any.
+    intros. by apply exclusive_local_update.
+  Qed.
+
+  Lemma update_mapping_new_locale ζ ζ' (R R1 R2 : gset $ fmrole M) m :
+    ζ' ∉ dom m ->
+    auth_mapping_is m -∗
+    ζ ↦M R ==∗
+    auth_mapping_is (<[ ζ' := R2]> (<[ ζ := R1 ]> m)) ∗
+    ζ ↦M R1 ∗ ζ' ↦M R2.
+  Proof.
+    iIntros (Hnotin) "Hamap Hmap".
+    iDestruct (mapping_lookup with "Hamap Hmap") as %Hin.
+    iCombine "Hamap Hmap" as "H".
+    iMod (own_update (A := (authUR (gmapUR _ (exclR (gsetR (RoleO M)))))) _ _ (
+                       ● ((λ f : gset (fmrole M), Excl f) <$> ((<[ ζ := R1 ]> m)))
+                         ⋅ ◯ ((λ f : gset (fmrole M), Excl f) <$> {[ζ := R1]})
+                     ) with "H") as "[A B]".
+    { rewrite !map_fmap_singleton fmap_insert.
+      eapply auth_update. eapply singleton_local_update_any.
+      intros. by apply exclusive_local_update. }
+    iCombine "A B" as "H".
+    iMod (own_update (A := (authUR (gmapUR _ (exclR (gsetR (RoleO M)))))) _ _ (
+                       ● ((λ f : gset (fmrole M), Excl f) <$> (<[ ζ' := R2]> (<[ ζ := R1 ]> m)))
+                         ⋅ ◯ ((λ f : gset (fmrole M), Excl f) <$> {[ζ := R1 ; ζ' := R2]})
+                     ) with "H") as "[A B]"; last first.
+    { iModIntro. iSplitL "A"; first iFrame. rewrite !fmap_insert fmap_empty insert_empty.
+      replace (◯ {[ζ := Excl R1; ζ' := Excl R2]}) with (◯ {[ζ := Excl R1]} ⋅ ◯ {[ζ' := Excl R2]}).
+      - iDestruct "B" as "[A B]". iSplitL "A"; rewrite /frag_mapping_is map_fmap_singleton //.
+      - rewrite -auth_frag_op insert_singleton_op //. rewrite lookup_singleton_ne //. set_solver. }
+    rewrite !map_fmap_singleton fmap_insert !fmap_insert.
+    rewrite (insert_commute _ _ _ (Excl R1) (Excl R2)); last set_solver.
+    eapply auth_update. rewrite fmap_empty. eapply alloc_local_update; eauto.
+    - rewrite lookup_insert_ne; last set_solver. apply not_elem_of_dom. set_solver.
+    - done.
+  Qed.
+
+  Lemma update_mapping_delete ζ (Rrem : gset $ fmrole M) (R: gset (fmrole M)) m :
+    auth_mapping_is m -∗ ζ ↦M R ==∗ auth_mapping_is (<[ ζ := R ∖ Rrem ]> m) ∗ ζ ↦M (R ∖ Rrem).
+  Proof.
+    eauto using update_mapping.
+  Qed.
+
+  Lemma update_mapping_add ζ (Radd : gset $ fmrole M) (R: gset (fmrole M)) m :
+    auth_mapping_is m -∗ ζ ↦M R ==∗ auth_mapping_is (<[ ζ := R ∪ Radd ]> m) ∗ ζ ↦M (R ∪ Radd).
+  Proof.
+    eauto using update_mapping.
+  Qed.
+
+
+  Lemma update_has_fuels ζ fs fs' F m :
+    let LR := (dom F ∪ dom fs') ∖ (dom fs ∖ dom fs') in
+    (fs ≠ ∅) ->
+    (dom fs' ∖ dom fs ∩ dom F = ∅) ->
+    has_fuels ζ fs -∗
+    auth_fuel_is F -∗
+    auth_mapping_is m ==∗
+    auth_fuel_is (fuel_apply fs' F LR) ∗
+    has_fuels ζ fs' ∗
+    auth_mapping_is (<[ ζ := dom fs' ]> m).
+  Proof.
+    iIntros (LR Hfs Hdom) "Hfuels Hafuels Hamapping".
+    rewrite !has_fuels_equiv. iDestruct "Hfuels" as "[Hmapping Hfuels]".    
+    iMod (update_fuel with "Hafuels Hfuels") as "[Hafuels Hfuels]" =>//.
+    iMod (update_mapping with "Hamapping Hmapping") as "[Hamapping Hmapping]".
+    iModIntro.
+    iFrame.
+  Qed.
+
+  Lemma update_has_fuels_no_step ζ fs fs' F m :
+    let LR := (dom F ∪ dom fs') ∖ (dom fs ∖ dom fs') in
+    (fs ≠ ∅) ->
+    (dom fs' ⊆ dom fs) ->
+    has_fuels ζ fs -∗
+    auth_fuel_is F -∗
+    auth_mapping_is m ==∗
+    auth_fuel_is (fuel_apply fs' F LR) ∗
+    has_fuels ζ fs' ∗
+    auth_mapping_is (<[ ζ := dom fs' ]> m).
+  Proof.
+    iIntros (LR Hfs Hdom) "Hfuels Hafuels Hamapping".
+    rewrite !has_fuels_equiv. iDestruct "Hfuels" as "[Hmapping Hfuels]".
+    iMod (update_fuel fs fs' with "Hafuels Hfuels") as "[Hafuels Hfuels]"; [done|set_solver|].
+    iMod (update_mapping with "Hamapping Hmapping") as "[Hamapping Hmapping]".
+    iModIntro. iFrame.
+  Qed.
+
+  Lemma update_has_fuels_no_step_no_change ζ fs fs' F m :
+    let LR := (dom F ∪ dom fs') ∖ (dom fs ∖ dom fs') in
+    (fs ≠ ∅) ->
+    (dom fs' = dom fs) ->
+    has_fuels ζ fs -∗
+    auth_fuel_is F -∗
+    auth_mapping_is m ==∗
+    auth_fuel_is (fuel_apply fs' F LR) ∗
+    has_fuels ζ fs' ∗
+    auth_mapping_is m.
+  Proof.
+    iIntros (LR Hfs Hdom) "Hfuels Hafuels Hamapping".
+    rewrite !has_fuels_equiv. iDestruct "Hfuels" as "[Hmapping Hfuels]".
+    iMod (update_fuel fs fs' with "Hafuels Hfuels") as "[Hafuels Hfuels]" =>//.
+    { rewrite Hdom. set_solver. }
+    iModIntro.
+    iFrame. rewrite Hdom //.
+  Qed.
+  
+End Updates.
